fe25519/fe25519_add.v
@@ -110,11 +110,11 @@ let            r3 :=  23%nat in
 let            r4 :=  24%nat in
 QCong
   (
-    (limbs 51 [::QVar x0; QVar x1; QVar x2; QVar x3; QVar x4])
+    (Radix51.limbs [::QVar x0; QVar x1; QVar x2; QVar x3; QVar x4])
     @+
-    (limbs 51 [::QVar y0; QVar y1; QVar y2; QVar y3; QVar y4])
+    (Radix51.limbs [::QVar y0; QVar y1; QVar y2; QVar y3; QVar y4])
   )
-  (limbs 51 [::QVar r0; QVar r1; QVar r2; QVar r3; QVar r4])
+  (Radix51.limbs [::QVar r0; QVar r1; QVar r2; QVar r3; QVar r4])
   (2^255 - 19).
 
 Definition fe25519_add_spec :=
@@ -124,11 +124,11 @@ Definition fe25519_add_spec :=
 
 Add Rec LoadPath "../lib/gbarith/src/" as GBArith.
 Add ML Path "../lib/gbarith/src/".
-From mathcomp Require Import eqtype ssrbool.
+From mathcomp Require Import ssreflect eqtype ssrbool.
 From mQhasm Require Import Verify.
 
 Lemma valid_fe25519_add : valid_ispec (fe25519_add_inputs, fe25519_add_spec).
 Proof.
   Time verify_ispec.
-  (* 52.519s *)
+  (* 30.461s *)
 Qed.
